Weidenbach_Book/IsaSAT_Setup.thy
@@ -1175,5 +1175,9 @@ lemma mop_polarity_st_heur_mop_polarity_wl'':
   by (rule fref_mono[THEN set_mp, OF _ _ _ mop_polarity_st_heur_mop_polarity_wl])
     (auto simp: \<L>\<^sub>a\<^sub>l\<^sub>l_all_atms_all_lits twl_st_heur'_def map_fun_rel_def)
 
+(* TODO Kill lhs*)
+lemma [simp,iff]: \<open>literals_are_\<L>\<^sub>i\<^sub>n (all_atms_st S) S \<longleftrightarrow> blits_in_\<L>\<^sub>i\<^sub>n S\<close>
+  unfolding literals_are_\<L>\<^sub>i\<^sub>n_def is_\<L>\<^sub>a\<^sub>l\<^sub>l_def \<L>\<^sub>a\<^sub>l\<^sub>l_all_atms_all_lits
+  by auto
 
 end
